{-# OPTIONS --without-K #-}

module Definition.Conversion.EqRelInstance where

open import Definition.Untyped
open import Definition.Typed
open import Definition.Typed.Properties
open import Definition.Typed.RedSteps
open import Definition.Typed.Weakening using (_∷_⊆_; wkEq)
open import Definition.Conversion
open import Definition.Conversion.Reduction
open import Definition.Conversion.Universe
open import Definition.Conversion.Stability
open import Definition.Conversion.Soundness
open import Definition.Conversion.Lift
open import Definition.Conversion.Conversion
open import Definition.Conversion.Symmetry
open import Definition.Conversion.Transitivity
open import Definition.Conversion.Weakening
open import Definition.Typed.EqualityRelation
open import Definition.Typed.Consequences.Syntactic
open import Definition.Typed.Consequences.Substitution
open import Definition.Typed.Consequences.Injectivity
open import Definition.Typed.Consequences.Equality
open import Definition.Typed.Consequences.Reduction

open import Tools.Nat
open import Tools.Product
import Tools.PropositionalEquality as PE


data _⊢_~_∷_ (Γ : Con Term) (k l A : Term) : Set where
  ↑ : ∀ {B} → Γ ⊢ A ≡ B → Γ ⊢ k ~ l ↑ B → Γ ⊢ k ~ l ∷ A

~-var : ∀ {x A Γ} → Γ ⊢ var x ∷ A → Γ ⊢ var x ~ var x ∷ A
~-var x =
  let ⊢A = syntacticTerm x
  in  ↑ (refl ⊢A) (var x PE.refl)

~-app : ∀ {f g a b F G Γ}
      → Γ ⊢ f ~ g ∷ Πₑ F ▹ G
      → Γ ⊢ a [conv↑] b ∷ F
      → Γ ⊢ f ∘ₑ a ~ g ∘ₑ b ∷ G [ a ]
~-app (↑ A≡B x) x₁ =
  let _ , ⊢B = syntacticEq A≡B
      B' , whnfB' , D = fullyReducible ⊢B
      ΠFG≡B' = trans A≡B (subset* (red D))
      H , E , B≡ΠHE = Π≡A ΠFG≡B' whnfB'
      F≡H , G≡E = injectivity (PE.subst (λ x → _ ⊢ _ ≡ x) B≡ΠHE ΠFG≡B')
      _ , ⊢f , _ = syntacticEqTerm (soundnessConv↑Term x₁)
  in  ↑ (substTypeEq G≡E (refl ⊢f))
        (app (PE.subst (λ x → _ ⊢ _ ~ _ ↓ x)
                       B≡ΠHE ([~] _ (red D) whnfB' x))
             (convConvTerm x₁ F≡H))

~-natrec : ∀ {z z' s s' n n' F F' Γ}
         → (Γ ∙ ℕₑ) ⊢ F [conv↑] F' →
      Γ ⊢ z [conv↑] z' ∷ (F [ zeroₑ ]) →
      Γ ⊢ s [conv↑] s' ∷ (Πₑ ℕₑ ▹ (F ▹▹ F [ sucₑ (var zero) ]↑)) →
      Γ ⊢ n ~ n' ∷ ℕₑ →
      Γ ⊢ natrecₑ F z s n ~ natrecₑ F' z' s' n' ∷ (F [ n ])
~-natrec x x₁ x₂ (↑ A≡B x₄) =
  let _ , ⊢B = syntacticEq A≡B
      B' , whnfB' , D = fullyReducible ⊢B
      ℕ≡B' = trans A≡B (subset* (red D))
      B≡ℕ = ℕ≡A ℕ≡B' whnfB'
      k~l' = PE.subst (λ x → _ ⊢ _ ~ _ ↓ x) B≡ℕ
                      ([~] _ (red D) whnfB' x₄)
      ⊢F , _ = syntacticEq (soundnessConv↑ x)
      _ , ⊢n , _ = syntacticEqTerm (soundness~↓ k~l')
  in  ↑ (refl (substType ⊢F ⊢n))
        (natrec x x₁ x₂ k~l')

~-sym : {k l A : Term} {Γ : Con Term} → Γ ⊢ k ~ l ∷ A → Γ ⊢ l ~ k ∷ A
~-sym (↑ A≡B x) =
  let ⊢Γ = wfEq A≡B
      B , A≡B' , l~k = sym~↑ (reflConEq ⊢Γ) x
  in  ↑ (trans A≡B A≡B') l~k

~-trans : {k l m A : Term} {Γ : Con Term}
        → Γ ⊢ k ~ l ∷ A → Γ ⊢ l ~ m ∷ A
        → Γ ⊢ k ~ m ∷ A
~-trans (↑ x x₁) (↑ x₂ x₃) =
  let ⊢Γ = wfEq x
      k~m , _ = trans~↑ (reflConEq ⊢Γ) x₁ x₃
  in  ↑ x k~m

~-wk : {k l A : Term} {ρ : Wk} {Γ Δ : Con Term} →
      ρ ∷ Δ ⊆ Γ →
      ⊢ Δ → Γ ⊢ k ~ l ∷ A → Δ ⊢ wk ρ k ~ wk ρ l ∷ wk ρ A
~-wk x x₁ (↑ x₂ x₃) = ↑ (wkEq x x₁ x₂) (wk~↑ x x₁ x₃)

~-conv : {k l A B : Term} {Γ : Con Term} →
      Γ ⊢ k ~ l ∷ A → Γ ⊢ A ≡ B → Γ ⊢ k ~ l ∷ B
~-conv (↑ x x₁) x₂ = ↑ (trans (sym x₂) x) x₁

~-to-conv : {k l A : Term} {Γ : Con Term} →
      Γ ⊢ k ~ l ∷ A → Γ ⊢ k [conv↑] l ∷ A
~-to-conv (↑ x x₁) = convConvTerm (lift~toConv↑ x₁) (sym x)

instance eqRelInstance : EqRelSet
eqRelInstance = eqRel _⊢_[conv↑]_ _⊢_[conv↑]_∷_
                      _⊢_~_∷_ ~-var ~-app ~-natrec
                      ~-sym ~-trans ~-conv ~-wk ~-to-conv
                      (λ x → liftConv (U-refl x))
                      (λ x → liftConv (ℕ-refl x))
                      (λ x → liftConvTerm (univ (ℕ x) (ℕ x) (ℕ-refl x)))
                      (λ x → liftConvTerm (zero-refl x))
                      symConv symConvTerm
                      transConv transConvTerm
                      reductionConv↑ reductionConv↑Term
                      wkConv↑ wkConv↑Term
                      soundnessConv↑ soundnessConv↑Term
                      convConvTerm univConv↑
                      (λ x → liftConvTerm (suc-cong x))
                      (λ x x₁ x₂ → liftConv (Π-cong x x₁ x₂))
                      (λ x x₁ x₂ →
                         let _ , F∷U , H∷U = syntacticEqTerm (soundnessConv↑Term x₁)
                             _ , G∷U , E∷U = syntacticEqTerm (soundnessConv↑Term x₂)
                             ⊢Γ = wfTerm F∷U
                             F<>H = univConv↑ x₁
                             G<>E = univConv↑ x₂
                             F≡H = soundnessConv↑ F<>H
                             E∷U' = stabilityTerm (reflConEq ⊢Γ ∙ F≡H) E∷U
                         in  liftConvTerm (univ (Π F∷U ▹ G∷U) (Π H∷U ▹ E∷U')
                                                (Π-cong x F<>H G<>E)))
                      (λ x x₁ x₂ x₃ x₄ x₅ → liftConvTerm (fun-ext x x₁ x₂ x₃ x₄ x₅))
