{-# OPTIONS --without-K #-}

module Definition.Typed.Consequences.Substitution where

open import Definition.Untyped
open import Definition.Untyped.Properties
open import Definition.Typed
open import Definition.Typed.Properties
open import Definition.Typed.EqRelInstance
open import Definition.Typed.Weakening as T
open import Definition.Typed.Consequences.Syntactic
open import Definition.LogicalRelation
open import Definition.LogicalRelation.Irrelevance
open import Definition.LogicalRelation.Properties
open import Definition.LogicalRelation.Substitution
open import Definition.LogicalRelation.Substitution.Properties
import Definition.LogicalRelation.Substitution.Irrelevance as S
open import Definition.LogicalRelation.Fundamental

open import Tools.Product
open import Tools.Unit
import Tools.PropositionalEquality as PE


substitution : ∀ {A Γ Δ σ} → Γ ⊢ A → Δ ⊢ₛ σ ∷ Γ → ⊢ Δ → Δ ⊢ subst σ A
substitution A σ ⊢Δ with fundamental A | fundamentalSubst (wf A) ⊢Δ σ
substitution A σ ⊢Δ | [Γ] , [A] | [Γ]' , [σ] =
  wellformed (proj₁ ([A] ⊢Δ (S.irrelevanceSubst [Γ]' [Γ] ⊢Δ ⊢Δ [σ])))

substitutionEq : ∀ {A B Γ Δ σ σ'}
               → Γ ⊢ A ≡ B → Δ ⊢ₛ σ ≡ σ' ∷ Γ → ⊢ Δ → Δ ⊢ subst σ A ≡ subst σ' B
substitutionEq A≡B σ ⊢Δ with fundamentalEq A≡B | fundamentalSubstEq (wfEq A≡B) ⊢Δ σ
substitutionEq A≡B σ ⊢Δ | [Γ] , [A] , [B] , [A≡B] | [Γ]' , [σ] , [σ'] , [σ≡σ']  =
  let [σ]' = S.irrelevanceSubst [Γ]' [Γ] ⊢Δ ⊢Δ [σ]
      [σ']' = S.irrelevanceSubst [Γ]' [Γ] ⊢Δ ⊢Δ [σ']
      [σ≡σ']' = S.irrelevanceSubstEq [Γ]' [Γ] ⊢Δ ⊢Δ [σ] [σ]' [σ≡σ']
  in  wellformedEq (proj₁ ([A] ⊢Δ [σ]'))
                   (transEq (proj₁ ([A] ⊢Δ [σ]')) (proj₁ ([B] ⊢Δ [σ]'))
                            (proj₁ ([B] ⊢Δ [σ']')) ([A≡B] ⊢Δ [σ]')
                            (proj₂ ([B] ⊢Δ [σ]') [σ']' [σ≡σ']'))

substitutionTerm : ∀ {t A Γ Δ σ}
               → Γ ⊢ t ∷ A → Δ ⊢ₛ σ ∷ Γ → ⊢ Δ → Δ ⊢ subst σ t ∷ subst σ A
substitutionTerm t σ ⊢Δ with fundamentalTerm t | fundamentalSubst (wfTerm t) ⊢Δ σ
substitutionTerm t σ ⊢Δ | [Γ] , [A] , [t] | [Γ]' , [σ] =
  let [σ]' = S.irrelevanceSubst [Γ]' [Γ] ⊢Δ ⊢Δ [σ]
  in  wellformedTerm (proj₁ ([A] ⊢Δ [σ]')) (proj₁ ([t] ⊢Δ [σ]'))

substitutionEqTerm : ∀ {t u A Γ Δ σ σ'}
                   → Γ ⊢ t ≡ u ∷ A → Δ ⊢ₛ σ ≡ σ' ∷ Γ → ⊢ Δ
                   → Δ ⊢ subst σ t ≡ subst σ' u ∷ subst σ A
substitutionEqTerm t≡u σ≡σ' ⊢Δ with fundamentalTermEq t≡u
                                  | fundamentalSubstEq (wfEqTerm t≡u) ⊢Δ σ≡σ'
... | [Γ] , modelsTermEq [A] [t] [u] [t≡u] | [Γ]' , [σ] , [σ'] , [σ≡σ'] =
  let [σ]' = S.irrelevanceSubst [Γ]' [Γ] ⊢Δ ⊢Δ [σ]
      [σ']' = S.irrelevanceSubst [Γ]' [Γ] ⊢Δ ⊢Δ [σ']
      [σ≡σ']' = S.irrelevanceSubstEq [Γ]' [Γ] ⊢Δ ⊢Δ [σ] [σ]' [σ≡σ']
  in  wellformedTermEq (proj₁ ([A] ⊢Δ [σ]'))
                       (transEqTerm (proj₁ ([A] ⊢Δ [σ]')) ([t≡u] ⊢Δ [σ]')
                                    (proj₂ ([u] ⊢Δ [σ]') [σ']' [σ≡σ']'))

substRefl : ∀ {σ Γ Δ}
          → Δ ⊢ₛ σ ∷ Γ
          → Δ ⊢ₛ σ ≡ σ ∷ Γ
substRefl id = id
substRefl (σ , x) = substRefl σ , refl x

wkSubst' : ∀ {ρ σ Γ Δ Δ'} (⊢Γ : ⊢ Γ) (⊢Δ : ⊢ Δ) (⊢Δ' : ⊢ Δ')
           ([ρ] : ρ ∷ Δ' ⊆ Δ)
           ([σ] : Δ ⊢ₛ σ ∷ Γ)
         → Δ' ⊢ₛ ρ •ₛ σ ∷ Γ
wkSubst' ε ⊢Δ ⊢Δ' ρ id = id
wkSubst' (_∙_ {Γ} {A} ⊢Γ ⊢A) ⊢Δ ⊢Δ' ρ (tailσ , headσ) =
  wkSubst' ⊢Γ ⊢Δ ⊢Δ' ρ tailσ
  , PE.subst (λ x → _ ⊢ _ ∷ x) (wk-subst A) (wkTerm ρ ⊢Δ' headσ)

wk1Subst' : ∀ {F σ Γ Δ} (⊢Γ : ⊢ Γ) (⊢Δ : ⊢ Δ)
            (⊢F : Δ ⊢ F)
            ([σ] : Δ ⊢ₛ σ ∷ Γ)
          → (Δ ∙ F) ⊢ₛ wk1Subst σ ∷ Γ
wk1Subst' {F} {σ} {Γ} {Δ} ⊢Γ ⊢Δ ⊢F [σ] =
  wkSubst' ⊢Γ ⊢Δ (⊢Δ ∙ ⊢F) (T.step T.id) [σ]

liftSubst' : ∀ {F σ Γ Δ} (⊢Γ : ⊢ Γ) (⊢Δ : ⊢ Δ)
             (⊢F  : Γ ⊢ F)
             ([σ] : Δ ⊢ₛ σ ∷ Γ)
           → (Δ ∙ subst σ F) ⊢ₛ liftSubst σ ∷ Γ ∙ F
liftSubst' {F} {σ} {Γ} {Δ} ⊢Γ ⊢Δ ⊢F [σ] =
  let ⊢Δ∙F = ⊢Δ ∙ substitution ⊢F [σ] ⊢Δ
  in  wkSubst' ⊢Γ ⊢Δ ⊢Δ∙F (T.step T.id) [σ]
  ,   var ⊢Δ∙F (PE.subst (λ x → 0 ∷ x ∈ (Δ ∙ subst σ F))
                         (wk-subst F) here)

idSubst' : ∀ {Γ} (⊢Γ : ⊢ Γ)
         → Γ ⊢ₛ idSubst ∷ Γ
idSubst' ε = id
idSubst' (_∙_ {Γ} {A} ⊢Γ ⊢A) =
  wk1Subst' ⊢Γ ⊢Γ ⊢A (idSubst' ⊢Γ)
  , PE.subst (λ x → Γ ∙ A ⊢ _ ∷ x) (wk1-tailId A) (var (⊢Γ ∙ ⊢A) here)

substComp' : ∀ {σ σ' Γ Δ Δ'} (⊢Γ : ⊢ Γ) (⊢Δ : ⊢ Δ) (⊢Δ' : ⊢ Δ')
             ([σ] : Δ' ⊢ₛ σ ∷ Δ)
             ([σ'] : Δ ⊢ₛ σ' ∷ Γ)
           → Δ' ⊢ₛ σ ₛ•ₛ σ' ∷ Γ
substComp' ε ⊢Δ ⊢Δ' [σ] id = id
substComp' (_∙_ {Γ} {A} ⊢Γ ⊢A) ⊢Δ ⊢Δ' [σ] ([tailσ'] , [headσ']) =
  substComp' ⊢Γ ⊢Δ ⊢Δ' [σ] [tailσ']
  , PE.subst (λ x → _ ⊢ _ ∷ x) (substCompEq A)
             (substitutionTerm [headσ'] [σ] ⊢Δ')

singleSubst : ∀ {A t Γ} → Γ ⊢ t ∷ A → Γ ⊢ₛ sgSubst t ∷ Γ ∙ A
singleSubst {A} t =
  let ⊢Γ = wfTerm t
  in  idSubst' ⊢Γ , PE.subst (λ x → _ ⊢ _ ∷ x) (PE.sym (subst-id A)) t

singleSubstEq : ∀ {A t u Γ} → Γ ⊢ t ≡ u ∷ A
              → Γ ⊢ₛ sgSubst t ≡ sgSubst u ∷ Γ ∙ A
singleSubstEq {A} t =
  let ⊢Γ = wfEqTerm t
  in  substRefl (idSubst' ⊢Γ) , PE.subst (λ x → _ ⊢ _ ≡ _ ∷ x) (PE.sym (subst-id A)) t

singleSubst↑ : ∀ {A t Γ} → Γ ∙ A ⊢ t ∷ wk1 A → Γ ∙ A ⊢ₛ consSubst (wk1Subst idSubst) t ∷ Γ ∙ A
singleSubst↑ {A} t with wfTerm t
... | ⊢Γ ∙ ⊢A = wk1Subst' ⊢Γ ⊢Γ ⊢A (idSubst' ⊢Γ)
              , PE.subst (λ x → _ ∙ A ⊢ _ ∷ x) (wk1-tailId A) t

singleSubst↑Eq : ∀ {A t u Γ} → Γ ∙ A ⊢ t ≡ u ∷ wk1 A
              → Γ ∙ A ⊢ₛ consSubst (wk1Subst idSubst) t ≡ consSubst (wk1Subst idSubst) u ∷ Γ ∙ A
singleSubst↑Eq {A} t with wfEqTerm t
... | ⊢Γ ∙ ⊢A = substRefl (wk1Subst' ⊢Γ ⊢Γ ⊢A (idSubst' ⊢Γ))
              , PE.subst (λ x → _ ∙ A ⊢ _ ≡ _ ∷ x) (wk1-tailId A) t

-- Helper lemmas for single substitution

substType : ∀ {t F G Γ} → Γ ∙ F ⊢ G → Γ ⊢ t ∷ F → Γ ⊢ G [ t ]
substType {t} {F} {G} ⊢G ⊢t =
  let ⊢Γ = wfTerm ⊢t
  in  substitution ⊢G (singleSubst ⊢t) ⊢Γ

substTypeEq : ∀ {t u F G E Γ} → Γ ∙ F ⊢ G ≡ E → Γ ⊢ t ≡ u ∷ F → Γ ⊢ G [ t ] ≡ E [ u ]
substTypeEq {F = F} ⊢G ⊢t =
  let ⊢Γ = wfEqTerm ⊢t
  in  substitutionEq ⊢G (singleSubstEq ⊢t) ⊢Γ

substTerm : ∀ {F G t f Γ} → Γ ∙ F ⊢ f ∷ G → Γ ⊢ t ∷ F → Γ ⊢ f [ t ] ∷ G [ t ]
substTerm {F} {G} {t} {f} ⊢f ⊢t =
  let ⊢Γ = wfTerm ⊢t
  in  substitutionTerm ⊢f (singleSubst ⊢t) ⊢Γ

substTypeΠ : ∀ {t F G Γ} → Γ ⊢ Πₑ F ▹ G → Γ ⊢ t ∷ F → Γ ⊢ G [ t ]
substTypeΠ ΠFG t with syntacticΠ ΠFG
substTypeΠ ΠFG t | F , G = substType G t

subst↑Type : ∀ {t F G Γ}
           → Γ ∙ F ⊢ G
           → Γ ∙ F ⊢ t ∷ wk1 F
           → Γ ∙ F ⊢ G [ t ]↑
subst↑Type ⊢G ⊢t = substitution ⊢G (singleSubst↑ ⊢t) (wfTerm ⊢t)

subst↑TypeEq : ∀ {t u F G E Γ}
             → Γ ∙ F ⊢ G ≡ E
             → Γ ∙ F ⊢ t ≡ u ∷ wk1 F
             → Γ ∙ F ⊢ G [ t ]↑ ≡ E [ u ]↑
subst↑TypeEq ⊢G ⊢t = substitutionEq ⊢G (singleSubst↑Eq ⊢t) (wfEqTerm ⊢t)
